src/program_proof/lockservice/common_proof.v
@@ -1,0 +1,70 @@
+From Perennial.program_proof.lockservice Require Import lockservice fmcounter_map rpc.
+From iris.program_logic Require Export weakestpre.
+From Perennial.goose_lang Require Import prelude.
+From Perennial.goose_lang Require Import ffi.disk_prelude.
+From Perennial.goose_lang Require Import notation.
+From Perennial.program_proof Require Import proof_prelude.
+From stdpp Require Import gmap.
+From RecordUpdate Require Import RecordUpdate.
+From Perennial.algebra Require Import auth_map fmcounter.
+From Perennial.goose_lang.lib Require Import lock.
+From Perennial.Helpers Require Import NamedProps.
+From Perennial.Helpers Require Import ModArith.
+From iris.algebra Require Import numbers.
+From Coq.Structures Require Import OrdersTac.
+Section lockservice_common_proof.
+
+Context `{!heapG Σ}.
+
+Axiom nondet_spec:
+  {{{ True }}}
+    nondet #()
+  {{{ v, RET v; ⌜v = #true⌝ ∨ ⌜v = #false⌝}}}.
+
+Lemma overflow_guard_incr_spec stk E (v:u64) : 
+{{{ True }}}
+  overflow_guard_incr #v @ stk ; E
+{{{
+     RET #(); ⌜((int.val v) + 1 = int.val (word.add v 1))%Z⌝
+}}}.
+Proof.
+  iIntros (Φ) "Hpre Hpost".
+  wp_lam. wp_pures.
+  wp_apply (wp_forBreak_cond
+              (fun b => ((⌜b = true⌝ ∨ ⌜((int.val v) + 1 = int.val (word.add v 1))%Z⌝)
+)) with "[] []")%I; eauto.
+  {
+    iIntros (Ψ). iModIntro.
+    iIntros "_ HΨpost".
+    wp_pures.
+    destruct bool_decide eqn:Hineq.
+    {
+      apply bool_decide_eq_true in Hineq.
+      wp_pures.
+      iApply "HΨpost".
+      iFrame; by iLeft.
+    }
+    {
+      apply bool_decide_eq_false in Hineq.
+      wp_pures.
+      iApply "HΨpost". iFrame; iRight.
+      iPureIntro.
+      assert (int.val (word.add v 1) >= int.val v)%Z by lia.
+      destruct (bool_decide ((int.val v) + 1 < 2 ^ 64 ))%Z eqn:Hnov.
+      {
+        apply bool_decide_eq_true in Hnov.
+        word.
+      }
+      apply bool_decide_eq_false in Hnov.
+      assert (int.val v + (int.val 1) >= 2 ^ 64)%Z.
+      { replace (int.val 1)%Z with (1)%Z by word. lia. }
+      apply sum_overflow_check in H0.
+      contradiction.
+    }
+  }
+  {
+    iIntros "[ %| %]"; first discriminate.
+    by iApply "Hpost".
+  }
+Qed.
+End lockservice_common_proof.
